(WIP) adds in spike, not yet removed previous detritus from Klon.dfy

Object.dfy
@@ -5,7 +5,7 @@
 type Owner = set<Object>   //still trying to devie if this sould be called Owner or Owners or Region or what!
 
 
-datatype Mode =   
+datatype Mode =
     | Rep // owned by me
     | Peer // owned by my owner
 //For all the Owner & Read "Modes" sholdn't the owner always be "self" i.e; the object containing the reernce.
@@ -13,7 +13,7 @@ datatype Mode =
     | Loaned(perm : Perm) //owning reference, but currently there are "borrowed" references to it
     | Borrow(perm: Perm, owner: Owner, from : Object, name : string) //borrowed reference, borrowe from that object!
                                       //when one does a "stack-pop-return" into the obejct that this was borrowed from
-                                      //then the Mode of the owning refernece goes from Loaned -> Owned 
+                                      //then the Mode of the owning refernece goes from Loaned -> Owned
     | Evil //type dyanmic.  So I don't hace to do the full checks right now --- kjx 7 May 2024
 
 
@@ -22,17 +22,17 @@ datatype Perm = Read | Write | Local   ///or should these be object kinds???>  A
 
     /// an earlier deprecated design!
     // | Own(perm : Owner) //unrestricted, Rust-style owning reference?
-    // | Read(owner : Owner) //Rust stule ownering Readonly reference? 
+    // | Read(owner : Owner) //Rust stule ownering Readonly reference?
     //                        //IF we have move semantics, could move here from Own?
     // | ReadOwn(owner : Owner)  // I am the owner, but my contents are read-borrowed.
     // | MutOwn(owner : Owner)  // I am the owner, but my contents are mut-borrowed.
     // | LocOwn(owner : Owner)  // I am the owner, but my contents are loc-borrowed.
-    // | ReadRef(owner : Owner) //       
+    // | ReadRef(owner : Owner) //
 
-predicate AssignmentCompatible(o : Object, t : Mode, v : Object) 
+predicate AssignmentCompatible(o : Object, t : Mode, v : Object)
 //can object v be assigned to a field of Mode t within object o?
 {
-  match t  
+  match t
     case Evil => true
     case Rep | Owned(_) | Loaned(_) => inside(v,o) //KJX is this right  hmm?
     case Peer => v.owner == o.owner
@@ -77,24 +77,24 @@ lemma EVILisCompatibleWithAnything(o : Object, v : Object)
 //
 //I know it's perverse, but titlecase "Object" (and "Class") aren't reserved in dafny
 //
-class Object { 
+class Object {
 
   const bound : Owner //movement bound - stands in for explcit owner parameters
   const AMFB  : Owner //flattened bound
 
   const owner : Owner//actual "dynamic" Owner owner of this object --- *XTERNAL*
-  const AMFX :  Owner//flattened owner  /// aka all externeal owners 
+  const AMFX :  Owner//flattened owner  /// aka all externeal owners
 
-  const ntrnl : Owner//actual "dynamic" internal region onwned by this object 
+  const ntrnl : Owner//actual "dynamic" internal region onwned by this object
   const AMFO  : Owner //All MY FUCKING Owner  (aka All My Flat Owner:-)
 
   var   fields     : map<string,Object>//field values. uninit fields have no entries
   var   fieldModes : map<string,Mode>//Mode of each field name -  note, static! - would be statically known by any methods
-    //probably also has to go to var to get to typestate. GRRR. 
+    //probably also has to go to var to get to typestate. GRRR.
 
   var nick : string //nickname
 
-  constructor make(ks : map<string,Mode>, oo : Owner, context : set<Object>, name : string, mb : Owner := oo) 
+  constructor make(ks : map<string,Mode>, oo : Owner, context : set<Object>, name : string, mb : Owner := oo)
     requires forall o <- oo :: o.Ready()  //hmmm
     requires oo >= mb
     requires CallOK(oo, context)
@@ -108,36 +108,38 @@ class Object {
 
 //    requires CallOK(flattenAMFOs(oo), context) //KJX is this right?
     requires CallOK(oo, context) //KJX is this right?
-  
+
     requires ownerInsideOwner(oo,mb)
 
     ensures owner == oo
     ensures AMFO == flattenAMFOs(oo) + {this}
     ensures bound == mb
     ensures AMFB == flattenAMFOs(mb) // + {this}  //HMM dunno if "this" should be here, but... --- ABSOLUTELY NOT!
-  
+
     ensures fieldModes == ks
-    ensures fields == map[] 
+    ensures fields == map[]
 
     ensures this  in AMFO
     ensures this !in owner
 
-    ensures (forall oo <- allExternalOwners() :: AMFO >= oo.AMFO)
-    ensures (forall o <-  AMFO :: inside(this, o))
-
     ensures OwnersValid()
     ensures Ready()
 
-                                                                                   
-    ensures COK(this, context+{this})                  
+    ensures (forall oo <- allExternalOwners() :: AMFO >= oo.AMFO)
+    ensures (forall o <-  AMFO :: inside(this, o))
+
+
+
+
+    ensures COK(this, context+{this})
     ensures nick == name
-  
+
     //ensures CallOK({this} + {oo}+oo.AMFO, {this} + context)
 
     ensures unchanged( context )
     ensures fresh(this)
 
-  { 
+  {
     bound := mb;
     AMFB  := flattenAMFOs(mb);// + {this}; -- see above
 
@@ -150,7 +152,12 @@ class Object {
     fieldModes := ks;
     fields := map[];
     nick := name;
-    new; 
+    new;
+
+// just can't be done here!!!
+// assert OwnersValid();
+// assert Ready();
+// assert (forall os <- allExternalOwners() :: AMFO >= os.AMFO);
 
     assert AMFX == AMFO - {this};
 
@@ -161,38 +168,38 @@ class Object {
     assert CallOK(oo, context);
     assert CallOK(context);
     CallOKAMFO(oo, context);
-    assert  (this in context+{this}) by { reveal COK(), CallOK(); } 
-    assert  (AMFO <= context+{this}) by { reveal COK(), CallOK(); } 
+    assert  (this in context+{this}) by { reveal COK(), CallOK(); }
+    assert  (AMFO <= context+{this}) by { reveal COK(), CallOK(); }
 
     assert CallOK(oo, context);
     CallOKWiderContext(oo, context,{this});
     assert CallOK(oo, context+{this});
 
   // assert CallOK(oo.AMFO, {this}+context) by { assert {this}+context == context+{this}; }
-  
 
-    assert COK(this, {this}+context) by 
-        { 
+
+    assert COK(this, {this}+context) by
+        {
           reveal COK();
-  
+
           assert (this in ({this}+context));
           assert (this.AMFO <= ({this}+context));
           RVfromCallOK(oo,context);
 
           assert (forall x <- owner, xo <- x.AMFO :: xo in x.AMFO);
-  
 
-          assert AMFO == flattenAMFOs(oo) + {this}; 
+
+          assert AMFO == flattenAMFOs(oo) + {this};
           assert this !in flattenAMFOs(oo);
           assert (forall a <- oo  :: a.Ready());     //why are these here?
-          assert (forall a <- oo  :: AMFO > a.AMFO); 
-  
-          // assert (forall oo  <- AMFO  :: AMFO > oo.AMFO); 
+          assert (forall a <- oo  :: AMFO > a.AMFO);
+
+          // assert (forall oo  <- AMFO  :: AMFO > oo.AMFO);
 
           assert (forall o <- (allExternalOwners()) :: o.Ready());
           assert (forall o <- (allExternalOwners()) :: AMFO > o.AMFO);
           assert (this.Ready());
-          assert (this.Valid()); 
+          assert (this.Valid());
           assert (this.AllOutgoingReferencesAreOwnership(({this}+context)))  ;
           assert (this.AllOutgoingReferencesWithinThisHeap(({this}+context)));
           assert (this.AllOwnersAreWithinThisHeap(({this}+context)));
@@ -207,11 +214,11 @@ class Object {
 
 
 
-  assert COKOK: COK(this, context+{this}) 
+  assert COKOK: COK(this, context+{this})
     by { assert  {this}+context == context+{this}; }
 
   CallOKfromCOK(this, {this}+context);
- 
+
   assert CallOK({this}, {this}+context);
 
   COKAMFO(oo, context);
@@ -224,7 +231,6 @@ assert CallOK(flattenAMFOs(oo),  {this} + context);
 
 
 
-assert (forall os <- allExternalOwners() :: AMFO >= os.AMFO);      
 
   assert CallOK({this} + flattenAMFOs(oo), {this} + context);
 
@@ -244,7 +250,7 @@ assert (forall os <- allExternalOwners() :: AMFO >= os.AMFO);
 
 
 
-  constructor fake(ks : map<string,Mode>, oo : Owner, context : set<Object>, name : string, mb : Owner := oo) 
+  constructor fake(ks : map<string,Mode>, oo : Owner, context : set<Object>, name : string, mb : Owner := oo)
   {
     owner := oo;
     bound := mb;
@@ -252,8 +258,8 @@ assert (forall os <- allExternalOwners() :: AMFO >= os.AMFO);
     fieldModes := ks;
     fields := map[];
     nick := name;
-    new;   
- 
+    new;
+
    // print "Object.fake() just constructed ", fmtobj(this), "\n";
   }
 
@@ -270,11 +276,11 @@ assert (forall os <- allExternalOwners() :: AMFO >= os.AMFO);
 
 
 
-lemma triceratops(aa : set<Object>, bb : set<Object>, cc : set<Object>) 
+lemma triceratops(aa : set<Object>, bb : set<Object>, cc : set<Object>)
   ensures (aa + bb + cc) == ((aa + bb) + cc) == (aa + (bb + cc))
 {}
 
-lemma noFieldsAreAlwaysGoodFields() 
+lemma noFieldsAreAlwaysGoodFields()
  requires fields == map[]
  ensures  AllFieldsAreDeclared()
  ensures  AllFieldsContentsConsistentWithTheirDeclaration()
@@ -282,7 +288,7 @@ lemma noFieldsAreAlwaysGoodFields()
 
 lemma flatOwnersConvariantOK1(xx : set<Object>, yy : set<Object>)
   requires AllTheseOwnersAreFlatOK(xx,xx+yy)
-  ensures  flattenAMFOs(xx) <= yy + xx 
+  ensures  flattenAMFOs(xx) <= yy + xx
 {
   reveal AllTheseOwnersAreFlatOK();
   assert AllTheseOwnersAreFlatOK(xx,xx+yy);
@@ -295,6 +301,10 @@ lemma flatOwnersConvariantOK2(xx : set<Object>, yy : set<Object>)
   assert AllTheseOwnersAreFlatOK(xx,xx+yy) == ( flattenAMFOs(xx) <= yy + xx );
 }
 
+lemma anoyingExternalOwners()
+  requires Ready()
+  ensures (forall os <- allExternalOwners() :: AMFO >= os.AMFO)
+{}
 
 
 
@@ -305,37 +315,46 @@ lemma flatOwnersConvariantOK2(xx : set<Object>, yy : set<Object>)
 
 
 
-
-
-/*opaque*/ predicate Ready() 
+/*opaque*/ predicate Ready()
 // ready means all the owenrs are (at least) ready...
 // I had to inline the defition --- see "//Ready()inlined"
 // WHO the fuck knows WHY?
 // update this, update that too.
 
-//it's important: this has *no*  readsclausew
-   decreases AMFO, 1  
+//it's important: this has *no*  reads clause!
+   reads {}
+   decreases AMFO, 20
 { OwnersValid() }
+
+
+
+lemma u(o : Object)
+  requires o.Ready()
+  ensures  o !in o.AMFB
+  ensures  o !in o.AMFX
+  ensures  o  in o.AMFO
+{}
+
 
 
 function allExternalOwners() : (rv : set<Object>)
  //all o's owners except o itself
-   ///ensures rv == AMFX 
-   { AMFO - {this} }
+  // decreases AMFO, 30
+   { AMFX }
 
 function allExternalBounds() : set<Object>
  //all o's
  {  AMFB  } //AMFB can't have "this" in it...
 
 
-///*opaque*/ 
+///*opaque*/
 predicate Valid()
   decreases |AMFO|
 //  reads ValidReadSet()`fields,  ValidReadSet()`fieldModes
    reads this`fields, this`fieldModes
      requires Ready()
   //ensures Valid() ==> g()
- // reads this, this`Owner, AMFO, fields.Values, AMFO`fields, AMFO`Owner, 
+ // reads this, this`Owner, AMFO, fields.Values, AMFO`fields, AMFO`Owner,
  //    (set o1 <- AMFO, o2 <- o1.fields.Values :: o2) //JESUS MARY AND JOSEPH AND THE WEE DONKEY
   {
     OwnersValid()
@@ -346,21 +365,21 @@ predicate Valid()
     AllFieldsContentsConsistentWithTheirDeclaration()
     //    &&
     //  (forall o <- AMFO :: recInside(this, o))     //recInside needs valid, OOPS.
-  //  //  && 
+  //  //  &&
     // AllOutgoingReferencesAreVenice()
   }
 
-  predicate AllFieldsAreDeclared() 
+  predicate AllFieldsAreDeclared()
     reads this`fields, this`fieldModes
     { fields.Keys <= fieldModes.Keys }
 
   predicate AllFieldsContentsConsistentWithTheirDeclaration()
     requires AllFieldsAreDeclared()
     reads this`fields, this`fieldModes
-    { 
+    {
       forall n <- fields :: AssignmentCompatible(this, fieldModes[n], fields[n])
     }
-  
+
   predicate AllOutgoingReferencesAreOwnership(os : set<Object>)
     reads this`fields//, fields.Values,  os//semi-evil
     requires Ready() // ||  TRUMP()
@@ -377,7 +396,7 @@ predicate Valid()
        outgoing() <= os
     }
 
-lemma NoFieldsAreGoodFields(context : set<Object>) 
+lemma NoFieldsAreGoodFields(context : set<Object>)
   requires fields == map[]
   requires Ready()
   ensures AllOutgoingReferencesAreOwnership(context)
@@ -394,7 +413,7 @@ lemma NoFieldsAreGoodFields(context : set<Object>)
     }
 
   function outgoing() : set<Object> reads this`fields { fields.Values }
-  function fieldNames() : set<string> reads this`fields { fields.Keys }    //WAS {  fieldModes.Keys } 
+  function fieldNames() : set<string> reads this`fields { fields.Keys }    //WAS {  fieldModes.Keys }
   function size() : nat reads this`fields { |outgoing()| }
 
 
@@ -405,21 +424,20 @@ reads this`fields, AMFO`fields
      (set o1 <- AMFO, o2 <- o1.fields.Values :: o2) //JESUS MARY AND JOSEPH AND THE WEE DONKEY
 }
 
-lemma ReadyGetsOwnersValid() 
+lemma ReadyGetsOwnersValid()
   requires Ready()
   ensures OwnersValid()
 {
   //////reveal Ready();
-assert OwnersValid(); 
+assert OwnersValid();
 }
 
 
 
 
-//KJX should refactor all these invariants
-predicate OwnersValid() : (rv : bool) //newe version with Ready {}Mon18Dec}
-  decreases AMFO, 0
-  ensures rv ==> (AMFO >= AMFB)
+predicate  OwnersValid() : (rv : bool) //newe version with Ready {}Mon18Dec2024}
+  decreases AMFO, 10
+  reads {}
   {
   && (AMFB == flattenAMFOs(bound))
   && (AMFX == flattenAMFOs(owner))
@@ -431,44 +449,65 @@ predicate OwnersValid() : (rv : bool) //newe version with Ready {}Mon18Dec}
   && (this !in AMFX)
   && (this  in AMFO)
 
-  && (AMFO > AMFX >= AMFB)
+  && (forall x <- AMFO, oo <- x.AMFO ::  AMFO >= oo.AMFO)
+  && (forall b <- AMFO, c <- b.AMFO :: c in AMFO && inside(b,c) && inside(this,c))
 
-  && (forall oo <- owner :: AMFO > oo.AMFO)
-  && (forall oo <- owner :: oo.Ready())
-  && (forall o <- AMFO :: inside(this, o))  // {todo could move   this out}
-  && (forall b <- AMFO, c <- b.AMFO :: c in AMFO && inside(b,c) && inside(this,c))  
-  && ownerInsideOwner(owner,bound)
-  && (allExternalOwners() == flattenAMFOs(owner) == AMFX)  //KJX hmmm again 
-  && (AMFX == AMFO - {this})
+  && (AMFO > AMFX >= AMFB)
+  && (owner >= bound)
 
 //  && (AMFB == flattenAMFOs(bound) + {this}) //WTFFF - how is thatPOSSIBLE - 20Dec2024
-// 
+//
   }
 
 
-lemma AMFOsisAMFOs() 
+lemma AMFOsisAMFOs()
    requires Ready()
    requires OwnersValid()
    ensures forall oo <- AMFO :: oo.AMFO <= AMFO
 {}
 
-lemma AMFOsisAMFOs2() 
+lemma AMFOsisAMFOs2()
    requires Ready()
    requires OwnersValid()
    ensures forall x <- AMFO, oo <- x.AMFO :: oo.AMFO <= AMFO
 {}
 
+lemma AMFOsisAMFOs3()
+   requires Ready()
+   requires OwnersValid()
+   ensures allExternalOwners() == flattenAMFOs(owner) == AMFX
+   ensures AMFO == (AMFX + {this})
+   ensures this in AMFO
+   ensures allExternalOwners() ==  AMFO - {this}
+   ensures this !in AMFX
+{}
+
+lemma AMFOsisAMFOs4()
+   requires Ready()
+   requires OwnersValid()
+ensures
+  && (forall oo <- owner :: AMFO > oo.AMFO)
+  && (forall oo <- AMFX  :: AMFO > oo.AMFO)
+  && (forall oo <- AMFO :: (oo != this) ==> (AMFO > oo.AMFO))
+  && (forall o <- AMFO :: inside(this, o))  // {todo could move   this out}
+  && (AMFX == AMFO - {this})
+  && (AMFO >= AMFB)
+
+{}
+
+
+
 
 lemma CallMyOwnersWillWitherAway(a : Object, context : set<Object>)
      //if CallOK(context) && COK(a,context)
-     //then my owners & AMFOs are all OK in context too 
+     //then my owners & AMFOs are all OK in context too
   requires CallOK(context)
-  requires (a in context) || (COK(a, context))  //umm why the || 
+  requires (a in context) || (COK(a, context))  //umm why the ||
 
   ensures  CallOK(a.owner, context)
   ensures  a.owner <= context  //should follow
-  ensures  a.AMFO <= context  //ditto, etc... 
-  ensures  forall oo <- a.AMFO :: COK(oo, context) //ditto - no idea if it's good to keep these or not. 
+  ensures  a.AMFO <= context  //ditto, etc...
+  ensures  forall oo <- a.AMFO :: COK(oo, context) //ditto - no idea if it's good to keep these or not.
   ensures  CallOK(a.AMFO, context)
 {
   reveal   CallOK();
@@ -476,12 +515,12 @@ lemma CallMyOwnersWillWitherAway(a : Object, context : set<Object>)
 }
 
 
-/*opaque*/ predicate TRUMP() ///*opaque*/ Valid() 
+/*opaque*/ predicate TRUMP() ///*opaque*/ Valid()
     reads this`fields, this`fieldModes
  //  reads ValidReadSet()`fields, ValidReadSet()`fieldModes
    { Ready() && Valid() }
 
-lemma BIDEN() 
+lemma BIDEN()
   requires TRUMP()
   ensures Ready() && Valid()
 {
@@ -501,18 +540,18 @@ lemma AllStandaloneMonotonic(aa : set<Object>, bb : set<Object>)
    //we have MOGO(aa);  SUPERMOGO(bb,aa+bb); ==> MOGO(aa+bb);
 ///note that there's *no* constraint saying aa !! bb
 
-  requires forall o <- (aa) :: (o.TRUMP())  
-  requires forall o <- (aa) :: (deTRUMP(o).AllOutgoingReferencesAreOwnership(aa))  
+  requires forall o <- (aa) :: (o.TRUMP())
+  requires forall o <- (aa) :: (deTRUMP(o).AllOutgoingReferencesAreOwnership(aa))
   requires forall o <- (aa) :: (o.AllOutgoingReferencesWithinThisHeap(aa))
   requires forall o <- (aa) :: (o.AllOwnersAreWithinThisHeap(aa))
 
-  requires forall o <- (bb) :: (o.TRUMP())  
-  requires forall o <- (bb) :: (deTRUMP(o).AllOutgoingReferencesAreOwnership(aa+bb))  
+  requires forall o <- (bb) :: (o.TRUMP())
+  requires forall o <- (bb) :: (deTRUMP(o).AllOutgoingReferencesAreOwnership(aa+bb))
   requires forall o <- (bb) :: (o.AllOutgoingReferencesWithinThisHeap(aa+bb))
   requires forall o <- (bb) :: (o.AllOwnersAreWithinThisHeap(aa+bb))
 
-  ensures  forall o <- (aa) :: (o.TRUMP())  
-  ensures  forall o <- (aa) :: (o.AllOutgoingReferencesAreOwnership(aa+bb))  
+  ensures  forall o <- (aa) :: (o.TRUMP())
+  ensures  forall o <- (aa) :: (o.AllOutgoingReferencesAreOwnership(aa+bb))
   ensures  forall o <- (aa) :: (o.AllOutgoingReferencesWithinThisHeap(aa+bb))
   ensures  forall o <- (aa) :: (o.AllOwnersAreWithinThisHeap(aa+bb))
 {
@@ -529,7 +568,7 @@ lemma AllStandaloneMonotonic(aa : set<Object>, bb : set<Object>)
    reads set o1 <- (AMFO + {this}), o2 <- o1.fields.Values :: o2`fieldModes
   //  reads set o1 <- (AMFO + {this}), o2 <- o1.ValidReadSet() :: o2
   //  reads (AMFO + {this}), (AMFO + {this})`fields
-  //  reads set o1 <- (AMFO + {this}), o2 <- o1.fields.Values :: o2 
+  //  reads set o1 <- (AMFO + {this}), o2 <- o1.fields.Values :: o2
   // ensures SUPERMAGA( {this} + AMFO, {this} + AMFO)   ///be nice, but I wannt make verythiug TRUMP?
 {
   //////reveal MOGO();
@@ -565,7 +604,7 @@ lemma AllStandaloneMonotonic(aa : set<Object>, bb : set<Object>)
    reads set o1 <- aa, o2 <- o1.fields.Values :: o2`fieldModes
   // ensures rv ==> SUPERMAGA(aa,aa)
 {
-  var res := 
+  var res :=
   && (forall o <- (aa) :: (o.TRUMP()))
   && (forall o <- (aa) :: (deTRUMP(o).AllOutgoingReferencesAreOwnership(aa))  )
   && (forall o <- (aa) :: (o.AllOutgoingReferencesWithinThisHeap(aa)))
@@ -583,7 +622,7 @@ assert true;
 //why in here, not in Ownerhsip.dfy?
 //why opaqie all of a sudden?
 // thisi  kind of SHITTY.
-// given one arg, yes they are all flat, 
+// given one arg, yes they are all flat,
 // given TWO args, checks all owners flatten witin context!!!
 opaque predicate AllTheseOwnersAreFlatOK(os : set<Object>, context : set<Object> := os)
 // true iff all os's AMFOS are inside os
@@ -607,13 +646,13 @@ lemma FlatAMFOsAreFlat(os : set<Object>, of : set<Object>, context : set<Object>
 
 
 
-predicate OrigBigfoot(os : set<Object>, context : set<Object> := os) 
+predicate OrigBigfoot(os : set<Object>, context : set<Object> := os)
 //os and the AMFO of every o in os are inside the context
-//alternative formulation of AllTheseOwnerAreFlatOK 
+//alternative formulation of AllTheseOwnerAreFlatOK
 {
   && (os <= context)
   && (forall o <- os :: o.AMFO <=  context)
-} 
+}
 
 predicate Bigfoot(os : set<Object>, context : set<Object> := os) : ( r : bool )
     ensures r ==> AllTheseOwnersAreFlatOK(os,context)
@@ -623,15 +662,15 @@ predicate Bigfoot(os : set<Object>, context : set<Object> := os) : ( r : bool )
 }
 
 
-//extra lemma pshychoBigFoot moved to Klon.dfy 
+//extra lemma pshychoBigFoot moved to Klon.dfy
 
-lemma SPLATTO(os : set<Object>, context : set<Object> := os)  
+lemma SPLATTO(os : set<Object>, context : set<Object> := os)
   ensures OrigBigfoot(os,context) == AllTheseOwnersAreFlatOK(os,context)
 {
   reveal AllTheseOwnersAreFlatOK();
 }
 
-lemma MaybeOrMaybeNot(o : Object, os : set<Object>) 
+lemma MaybeOrMaybeNot(o : Object, os : set<Object>)
 //does it matter of we care if "this" is in the set of AMFO's we're flattening?
 //I dob't think so, as long as it's OK...?
 //or rather, if os are OKJ, o.AMFO <= os, os+o are OK too...
@@ -645,11 +684,14 @@ lemma MaybeOrMaybeNot(o : Object, os : set<Object>)
 
 /*oopaque or not or both */
 function flattenAMFOs(os : set<Object>) : (of : set<Object>)
-   //flattened set of os.AMFO 
+   //flattened set of os.AMFO
    //earlier version required o in all objects AMFS, that's gone now
    //could put it back, require os to be Ready, or remove the os+ below
    //currently going with the version with fewer requirements...
    //requires forall o <- os :: o in o.AMFO  //not needed adding
+   ensures os <= of
+   ensures of >= os
+   ensures forall o <- os :: o.AMFO <= of
 {
     os +   ///not technically needed if we keep "requires forall o <- os :: o in o.AMFO"
     (set o <- os, oo <- o.AMFO :: oo)
@@ -668,7 +710,7 @@ lemma AMFOisBigger(o : Object)
 //GRRRR
 // lemma EitherWayIsFlat(a : Object, rrm : Map, amx : set<Object>)
 //   //requires rrm.calid()
-//   requires forall o <- a.extra, oo <- o.AMFO :: 
+//   requires forall o <- a.extra, oo <- o.AMFO ::
 //           && o in rrm.m.Keys
 //           && oo in rrm.m.Keys
 //           && rrm.m[o]  in amx
@@ -681,7 +723,7 @@ lemma AMFOisBigger(o : Object)
 
 
 
-lemma Splurge(o : Object, context : set<Object>) 
+lemma Splurge(o : Object, context : set<Object>)
   requires COK(o, context)
 
   ensures  forall oo <- (o.AMFO - {o}) :: o.AMFO > oo.AMFO
@@ -703,8 +745,8 @@ lemma Splurge(o : Object, context : set<Object>)
   predicate  {:vcs_split_on_every_assert}{:timeLimit 10} StandaloneObjectsAreValid(os : set<Object>) //do we know if "os" is "closed"?
     // reads set o <- os, rd <- ({o} + o.fields.Values) :: rd
   //  requires OutgoingReferencesAreInTheseObjects(os)   ///why is this needed now?
-  
-    //requires os <= objects   
+
+    //requires os <= objects
     //reads this, objects
     requires forall o <- os :: o.Ready() && o.Valid()
     reads os,  os`fields//, os`Owner //os`AMFO,
@@ -718,12 +760,12 @@ lemma Splurge(o : Object, context : set<Object>)
 
     //reads objects`fields, objects`Owner // objects`AMFO,
     {
-     forall o <- os :: StandaloneObjectIsValid(o,os) 
+     forall o <- os :: StandaloneObjectIsValid(o,os)
     }
 
 
 // todo: rename with a "withinthisheap" or something?
-predicate {:todo "really todo - add in other cases"}  StandaloneObjectIsValid(o : Object, os : set<Object>) 
+predicate {:todo "really todo - add in other cases"}  StandaloneObjectIsValid(o : Object, os : set<Object>)
    reads o`fields, o`fieldModes
    reads os`fields, os`fieldModes
   //  reads os, o, o.ValidReadSet()
@@ -732,7 +774,7 @@ predicate {:todo "really todo - add in other cases"}  StandaloneObjectIsValid(o 
    requires forall o <- os :: o.Ready() && o.Valid()
     {
        && (o.Valid())
-       && (o.AllOutgoingReferencesAreOwnership(os))  
+       && (o.AllOutgoingReferencesAreOwnership(os))
 //       && (o.AllOutgoingReferencesWithinThisHeap(os))
 //       && (o.AllOwnersAreWithinThisHeap(os))
     }
@@ -740,33 +782,33 @@ predicate {:todo "really todo - add in other cases"}  StandaloneObjectIsValid(o 
 
 
 
-predicate OutgoingReferencesAreInTheseObjects(os : set<Object>) 
+predicate OutgoingReferencesAreInTheseObjects(os : set<Object>)
       reads os
       //note that this is within *this objectset
       //see also OutgoingReferencesAreInThisHeap
 {
-     (forall o <- os :: o.outgoing() <= os) 
+     (forall o <- os :: o.outgoing() <= os)
 }
 
-predicate OutgoingHeapReferencesAreInTheseObjects(os : set<Object>) 
+predicate OutgoingHeapReferencesAreInTheseObjects(os : set<Object>)
       reads os
 {
 //      (forall f <- os, t <- f.outgoing() :: t in os )
-      (forall f <- os :: f.outgoing() <= os ) 
+      (forall f <- os :: f.outgoing() <= os )
 
 }
 
-predicate OutgoingReferencesFromTheseObjectsAreToTheseObjects(fs : set<Object>, ts : set<Object>) 
+predicate OutgoingReferencesFromTheseObjectsAreToTheseObjects(fs : set<Object>, ts : set<Object>)
       reads fs
 {
-     (forall f <- fs :: f.outgoing() <= ts) 
+     (forall f <- fs :: f.outgoing() <= ts)
 }
 
-predicate OutgoingHeapReferencesFromTheseObjectsAreToTheseObjects(fs : set<Object>, ts : set<Object>) 
+predicate OutgoingHeapReferencesFromTheseObjectsAreToTheseObjects(fs : set<Object>, ts : set<Object>)
       reads fs
 {
-//     (forall f <- fs, t <- f.outgoing() :: t in ts ) 
-     (forall f <- fs :: f.outgoing() <= ts) 
+//     (forall f <- fs, t <- f.outgoing() :: t in ts )
+     (forall f <- fs :: f.outgoing() <= ts)
 }
 
 
@@ -789,7 +831,7 @@ lemma NoIncomingReferencesMeansNoOutgoingReferences(o : Object, os : set<Object>
 
 
     //attempt at contradiction
-    if (exists e <- es :: e.t == o) 
+    if (exists e <- es :: e.t == o)
     {
       var e :|  e in es && e.t == o;
       assert e in es;
@@ -803,7 +845,7 @@ lemma NoIncomingReferencesMeansNoOutgoingReferences(o : Object, os : set<Object>
     edgesWork(os,es);
     edgesWorks2(os,es);
     assert ObjectsToEdges(os,es);
-   
+
     assert forall x <- os :: o !in x.outgoing();
 
    }
@@ -815,21 +857,21 @@ lemma NoIncomingReferencesMeansNoOutgoingReferences(o : Object, os : set<Object>
 
 lemma RefCountDistributesOverDisjointEdges(oo : set<Object>, aa : set<Edge>, bb : set<Edge>)
       requires aa !! bb
-      ensures 
+      ensures
        forall i <- oo ::
          refCountEdges(i, aa + bb) == refCountEdges(i, aa) + refCountEdges(i, bb)
-       ensures 
+       ensures
        forall i <- oo ::
          incomingEdges(i, aa + bb) == incomingEdges(i, aa) + incomingEdges(i, bb)
     {
       //calc == {
-       assert forall i <- oo :: 
+       assert forall i <- oo ::
             (set e <- aa | e.t == i) + (set e <- bb | e.t == i)
-            == (set e <- (aa+bb) | e.t == i); 
-       assert forall i <- oo :: 
+            == (set e <- (aa+bb) | e.t == i);
+       assert forall i <- oo ::
             incomingEdges(i,aa) + incomingEdges(i,bb)
             == incomingEdges(i,aa+bb);
-       assert forall i <- oo :: 
+       assert forall i <- oo ::
             refCountEdges(i,aa) + refCountEdges(i,bb)
             == refCountEdges(i,aa+bb);
       //}
@@ -838,7 +880,7 @@ lemma RefCountDistributesOverDisjointEdges(oo : set<Object>, aa : set<Edge>, bb 
 
 
 
-lemma ClosedHeapContainsAllFieldValues(os : set<Object>) 
+lemma ClosedHeapContainsAllFieldValues(os : set<Object>)
   requires OutgoingReferencesAreInTheseObjects(os)
   ensures allFieldValues(os) <= os
   {}
@@ -848,7 +890,7 @@ lemma ClosedHeapContainsAllFieldValues(os : set<Object>)
 //xs old objectset
 //f n t - assignment.
 //f.n not in xs
-twostate lemma edgeFUCKINGassignment(os : set<Object>, 
+twostate lemma edgeFUCKINGassignment(os : set<Object>,
       rs : set<Edge>, rn : set<Edge>,
                             f : Object, n : string, t : Object)
   //reads f`fieldModes
@@ -857,16 +899,16 @@ twostate lemma edgeFUCKINGassignment(os : set<Object>,
   requires n !in old(f.fields)
   requires t in os
   requires rs == old(edges(os))
-  requires rn ==     edges(os) 
-  //permits f == t or f != t 
-  requires forall o <- os :: 
-           forall m <- old(o.fields) :: 
+  requires rn ==     edges(os)
+  //permits f == t or f != t
+  requires forall o <- os ::
+           forall m <- old(o.fields) ::
              m in o.fields && o.fields[m] == old( o.fields[m] )
   requires forall o <- os :: unchanged(o`fieldModes)
-          //  forall m <- old(o.fieldModes) :: 
+          //  forall m <- old(o.fieldModes) ::
           //    m in o.fieldModes && o.fieldModes[m] == old( o.fieldModes[m] )
-  requires forall o <- (os) :: 
-           forall m <- (o.fields) :: 
+  requires forall o <- (os) ::
+           forall m <- (o.fields) ::
              ( (m in old(o.fields) && o.fields[m] == old( o.fields[m] ))
                  || (o == f && m == n &&  o.fields[m] == t)
              )
@@ -881,7 +923,7 @@ twostate lemma edgeFUCKINGassignment(os : set<Object>,
 
 lemma HeyFUCKOFF(x : Object, y : Object, zz : set<Object>)
   requires x in zz+{y}
-  requires x != y 
+  requires x != y
   ensures  x in zz
 {}
 
@@ -899,12 +941,12 @@ function allFieldValues(os : set<Object>) : set<Object>
 set o <- os, v <- o.fields.Values :: v
 }
 
-twostate lemma allFieldValuesUnchangedObject(o : Object) 
+twostate lemma allFieldValuesUnchangedObject(o : Object)
   requires unchanged(old(o.fields.Values))
   ensures unchanged(old(allFieldValues({o})))
 {}
 
-twostate lemma allFieldValuesUnchanged(os : set<Object>) 
+twostate lemma allFieldValuesUnchanged(os : set<Object>)
   requires forall o <- os :: unchanged(old(o.fields.Values))
   ensures unchanged(old(allFieldValues(os)))
 {
@@ -916,21 +958,3 @@ function allFieldValuesExcept(os : set<Object>, xo : Object) : set<Object>
 {
 set o <- os, v <- o.fields.Values | o != xo :: v
 }
-
-
-
-
-
-
-
-
-
-
-
-
-
-
-
-
-
-
