Ownership.dfy
@@ -7,43 +7,49 @@
 //////////////////////////////////////////////////////////////////////////////
 //////////////////////////////////////////////////////////////////////////////
 
-function owners(o : Object) : set<Object>
-// deprecated
- //all o's owners except o itself
- { o.allExternalOwners() } //should this be a function on objects? - 'tis now
+// function owners(o : Object) : set<Object>
+// // deprecated
+//  //all o's owners except o itself
+//  { o.allExternalOwners() } //should this be a function on objects? - 'tis now
 
 ///inside or equal to
 predicate inside(part : Object, whole : Object) : (rv : bool)
- // reads part, whole 
   ensures rv <==> (whole.AMFO <= part.AMFO)
- {
-   part.AMFO >= whole.AMFO
- }
+  {
+    part.AMFO >= whole.AMFO
+  }
 
 predicate outside(part : Object, whole : Object) : (rv : bool)
-  ensures rv <==> (not(inside(part,whole))) 
+  ensures rv <==> (not(inside(part,whole)))
   ensures rv <==> (not(part.AMFO >= whole.AMFO))
-  { 
+  {
     not(inside(part,whole))
   }
 
-///inside BUT NOT equal to
-predicate strictlyInside(part : Object, whole : Object) : (rv : bool)
- // reads part, whole 
- {
-// || whole.region.World?
-  && part != whole
-  && whole.AMFO <= part.AMFO
- }
+// ///inside BUT NOT equal to
+// predicate strictlyInside(part : Object, whole : Object) : (rv : bool)
+//  // reads part, whole
+//  {
+// // || whole.region.World?
+//   && part != whole
+//   && whole.AMFO <= part.AMFO
+//  }
+// lemma reallyStrictlyInside(part : Object, whole : Object)
+//  ensures strictlyInside(part, whole) == (part.AMFO > whole.AMFO) {}
 
 predicate directlyInside(part : Object, whole : Object) : (rv : bool)
  {
    whole.AMFO == part.allExternalOwners()  //?yeah - what if there are stack owners around?
  }
 
+lemma reallyDirectlyInside(part : Object, whole : Object)
+ ensures directlyInside(part, whole) == (part.AMFX == whole.AMFO) {}
+
+
+
 predicate directlyBounded(part : Object, bound : Object) : (rv : bool)
  {
-   (part.AMFB - {part})  == bound.AMFO //?yeah - what if there are stack owners around?
+   part.AMFB  == bound.AMFO //?yeah - what if there are stack owners around?
  }
 
  predicate insideOwner(part : Object, whole : Object) : (rv : bool)
@@ -53,7 +59,8 @@ predicate directlyBounded(part : Object, bound : Object) : (rv : bool)
   ensures rv <==> (whole.allExternalOwners() <= part.AMFO)
   ensures rv <==> (ownerInsideOwner(part.AMFO, whole.allExternalOwners()))
  {
-  part.AMFO >= whole.allExternalOwners()
+   part.AMFO >= whole.AMFX
+ //  part.AMFO >= whole.allExternalOwners()
 //    whole.allExternalOwners() <= part.AMFO
  }
 
@@ -70,7 +77,7 @@ predicate directlyBounded(part : Object, bound : Object) : (rv : bool)
 
 
 
-lemma InsideOwnerVsBound(part : Object, whole : Object, context : set<Object>) 
+lemma InsideOwnerVsBound(part : Object, whole : Object, context : set<Object>)
   requires COK(part, context)
   requires COK(whole, context)
   requires boundInsideOwner(part, whole)
@@ -83,31 +90,33 @@ lemma InsideOwnerVsBound(part : Object, whole : Object, context : set<Object>)
 //////////////////////////////////////////////////////////////////////////
 //////////////////////////////////////////////////////////////////////////
 // generalised verisons as required by "cut" -- hmm I feel unconvined by this
-////////////////////////////////////////////////////////////////////////// 
+//////////////////////////////////////////////////////////////////////////
 //////////////////////////////////////////////////////////////////////////
 
-predicate ownerInsideOwner(partO : Owner, wholeO : Owner) 
+predicate ownerInsideOwner(partO : Owner, wholeO : Owner)
 {
  partO >= wholeO
 }
 
 
-predicate ownerInsideOwnerInsideOwner(partO : Owner, midO : Owner, wholeO : Owner) 
+predicate ownerInsideOwnerInsideOwner(partO : Owner, midO : Owner, wholeO : Owner)
 {
 //  forall p <- partO :: exists w <- wholeO :: inside(p, w)
  partO >= midO >= wholeO
 }
 
 
-lemma BLURareCUNTS(partO : Owner, wholeO : Owner) 
-  requires ownerInsideOwner(partO, wholeO) 
+lemma BLURareCUNTS(partO : Owner, wholeO : Owner)
+  requires ownerInsideOwner(partO, wholeO)
   // ensures  not(partO !! wholeO)
-  // ensures  flattenAMFOs(partO) >= flattenAMFOs(wholeO) 
+  // ensures  flattenAMFOs(partO) >= flattenAMFOs(wholeO)
 {
 
 }
 
 lemma InsideToOwners(part : Object, whole : Object)
+ requires part.Ready()
+ requires whole.Ready()
  ensures inside(part,whole) == ownerInsideOwner(part.AMFO, whole.AMFO)
  ensures insideOwner(part,whole) == ownerInsideOwner(part.AMFO,whole.allExternalOwners())
  ensures inside(part,whole) ==> insideOwner(part,whole)
@@ -116,12 +125,12 @@ lemma InsideToOwners(part : Object, whole : Object)
 }
 
 
-//pretty nice version... {:Mon18Dec} 
+//pretty nice version... {:Mon18Dec}
 lemma transitiveInsideOwners(a : Owner, b : Owner, c : Owner)
   // requires a != b
   // requires b != c
   // requires c != a
-  //requires a.Valid() && b.Valid() && c.Valid()
+  //requires a.Ready() && b.Ready() && c.Ready()
   //requires forall o <- {a, b, c} :: o.region.Heap?
   //equires a.Ready() && b.Ready() && c.Ready()
 
@@ -136,10 +145,10 @@ lemma transitiveInsideOwners(a : Owner, b : Owner, c : Owner)
 ///put WORLD in every object's ownershiplist (AMFO alongwith itself)
 ///this this is simply t.owner in f.AMFO
 
-lemma PointingLemmaOld(f : Object, t : Object) 
+lemma PointingLemmaOld(f : Object, t : Object)
   requires t.owner <= (f.AMFB)
   requires boundInsideOwner(f, t)
-  ensures refOK(f,t)            
+  ensures refOK(f,t)
 {
   //KJX is this right?4
 
@@ -148,19 +157,19 @@ lemma PointingLemmaOld(f : Object, t : Object)
 }
 
 
-lemma PointingLemma(f : Object, t : Object) 
+lemma PointingLemma(f : Object, t : Object)
   requires boundInsideOwner(f, t)
-//    requires ownerInsideOwner(t.AMFO,  f.bound) 
-  ensures  refOK(f,t)            
+//    requires ownerInsideOwner(t.AMFO,  f.bound)
+  ensures  refOK(f,t)
 {
 }
 
 
-///OUTGOING requires something like 
+///OUTGOING requires something like
 ///if T is outside f (or outside F.owner)???
-///the T must be on f's putoing list. 
-///needs to be consistent up the hierarcy 
-  
+///the T must be on f's putoing list.
+///needs to be consistent up the hierarcy
+
 
 // lemma MOREreffing(f : Object, t : Object)
 //   ensures(refOK(f,t) <==> (boundInsideOwner(f, t) || (f==t)))
@@ -178,7 +187,7 @@ predicate OLDERrefOK(f : Object, t : Object) : (rv : bool)
 predicate oldishRefOK(f : Object, t : Object) : (rv : bool) //moved 23Dec2024
   { boundInsideOwner(f,t) || directlyInside(t,f) }
 
-predicate   refOK(f : Object, t : Object) : (rv : bool)
+predicate   oldyRefOK(f : Object, t : Object) : (rv : bool)
   // requires ownersOK(f,os) //isthere an AMFO verison of this? //this is snow the AMFO version
   // requires ownersOK(t,os)
   // reads f, t//, t`region
@@ -188,25 +197,27 @@ predicate   refOK(f : Object, t : Object) : (rv : bool)
   // ownerInsideOwner(f.AMFO,t.allExternalOwners())
   //ownerInsideOwner(part.AMFO, whole.allExternalOwners())
   //  ownerInsideOwner(f.bound,t.allExternalOwners())
-  (f==t) || 
-  boundInsideOwner(f,t) || directlyInside(t,f)
+  || (f==t)
+  || boundInsideOwner(f,t)
+  || directlyInside(t,f)
 }
+
 
 lemma WorldCanFuckItself(f : Object, t : Object)
 //we don't really have "world" any more but if we did...
   requires f.AMFO == {f}
   requires refOK(f,t)
-{ 
+{
   if (t.AMFO == {}) { assert refOK(f,t); return;}
   if (t.allExternalOwners() == {f})  { assert refOK(f,t); return;}
 }
 
-//pretty nice version... {:Mon18Dec 2023} 
+//pretty nice version... {:Mon18Dec 2023}
 lemma transitiveInside(a : Object, b : Object, c : Object)
   // requires a != b
   // requires b != c
   // requires c != a
-  //requires a.Valid() && b.Valid() && c.Valid()
+  //requires a.Ready() && b.Ready() && c.Ready()
   //requires forall o <- {a, b, c} :: o.region.Heap?
   requires a.Ready() && b.Ready() && c.Ready()
   requires inside(a,b)
@@ -254,7 +265,7 @@ lemma insideMyDirectOwner(a : Object)
 //a truncated eversiversion of transitiveinside
 //that's sticking around for auld lang syne?
 //a is inside some object c
-//a != c 
+//a != c
 //b is a's direct owner
 //b != c
 //b is insidde c
@@ -296,7 +307,7 @@ function ownersBetween(part : Object, whole : Object) : (rv : set<Object>)
 
 
 
-lemma ownershipIsMonotonic(a : Object, b : Object, c : set<Object>) 
+lemma ownershipIsMonotonic(a : Object, b : Object, c : set<Object>)
   requires a != b //oops!`
   requires a in c
   requires b in c
@@ -304,21 +315,27 @@ lemma ownershipIsMonotonic(a : Object, b : Object, c : set<Object>)
   requires COK(b,c)
   requires CallOK(c)
 
+  requires a.Ready() && b.Ready()
+  requires forall o <- c :: o.Ready()
+
 //  ensures (a in b.AMFO) ==> (b !in a.AMFO)
   requires a  in b.AMFO
-  ensures  b !in a.AMFO   
+  ensures  b !in a.AMFO
 {
  reveal COK(), CallOK();
- assert COK(a,c);  
- assert COK(b,c); 
+ assert COK(a,c);
+ assert COK(b,c);
  assert CallOK(c);
+
+a.AMFOsisAMFOs4();
+b.AMFOsisAMFOs4();
 
  assert forall o <- a.AMFO :: (o != a) ==> (a.AMFO > o.AMFO);
  assert forall o <- b.AMFO :: (o != b) ==> (b.AMFO > o.AMFO);
 
 
  assert a in b.AMFO;
- 
+
 
  assert b !in a.AMFO;
 }
@@ -340,7 +357,7 @@ lemma OwnersAreOutsideFuckers(a : Object, o : Object)
 
 
 
-lemma IAmInsideMyOwnersAndAMFO(a : Object, o : Object) 
+lemma IAmInsideMyOwnersAndAMFO(a : Object, o : Object)
     requires a.Ready() && a.Valid()
     requires o.Ready() && o.Valid()
     requires inside(a,o)
@@ -348,3 +365,58 @@ lemma IAmInsideMyOwnersAndAMFO(a : Object, o : Object)
     ensures  forall oo <- a.owner :: inside(a, oo)
 {
 }
+
+
+
+
+
+
+
+
+
+//////////////////////////////////////////////////////////////////////////////
+/// refOK -
+//////////////////////////////////////////////////////////////////////////////
+
+
+predicate refBI(f : Object, t : Object) {f.AMFB >= t.AMFX}
+predicate refDI(f : Object, t : Object) {f.AMFO == t.AMFX}
+predicate refOK(f : Object, t : Object) {(f==t) || refBI(f,t) || refDI(f,t)}
+
+
+
+///// lemmata
+
+lemma reallyRefOK(f : Object, t : Object)
+  ensures refOK(f,t) == oldyRefOK(f,t)
+  ensures refBI(f,t) == boundInsideOwner(f,t)
+  ensures refDI(f,t) == directlyInside(t,f)
+{}
+
+lemma bixy(a : Object, b : Object, c : Object, m : Klon)
+  requires a.Ready()
+  requires b.Ready()
+  requires c.Ready()
+
+//  requires forall o <- {a, b, c} :: o.Ready()  //doesn't wwork!
+
+  requires refBI(a,b)
+
+  ensures  (a.AMFO > a.AMFX >= a.AMFB)
+  ensures  (b.AMFO > b.AMFX >= b.AMFB)
+  ensures  a.AMFB >= b.AMFX
+  ensures  (a.AMFO > a.AMFX >= a.AMFB >= b.AMFX >= b.AMFB)
+  ensures  a.AMFB >= b.AMFB
+
+  //  Inside3(a,b,c);
+{}
+
+lemma trexy(a : Object, b : Object, c : Object, m : Klon)
+  requires a.Ready()
+  requires b.Ready()
+  requires c.Ready()
+
+  requires refBI(a,b)
+  requires refBI(b,c)
+  ensures  refBI(a,c)
+{}
